函数
\[
f(x)=\ln\frac{ax^2+7}{bx+3}=\ln(ax^2+7)-\ln(bx+3)
\]

### (1) 求 \(f'(2)\)
\[
f'(x)=\frac{2ax}{ax^2+7}-\frac{b}{bx+3}
\]
代入 \(x=2\)：
\[
f'(2)=\frac{4a}{4a+7}-\frac{b}{2b+3}
\]
故
\[
[A]=4,\ [B]=4,\ [C]=7,\ [D]=2,\ [E]=3
\]

### (2) \(x=2\) 处极小值为 0
极小值为 0 至少满足
\[
f(2)=0,\quad f'(2)=0
\]

先由 \(f(2)=0\)：
\[
\ln\frac{4a+7}{2b+3}=0 \Rightarrow \frac{4a+7}{2b+3}=1
\Rightarrow 4a+7=2b+3
\Rightarrow b=2a+2
\]

再由 \(f'(2)=0\)：
\[
\frac{4a}{4a+7}=\frac{b}{2b+3}
\]
代入 \(b=2a+2\)，注意 \(2b+3=4a+7\)，于是
\[
\frac{4a}{4a+7}=\frac{2a+2}{4a+7}
\Rightarrow 4a=2a+2
\Rightarrow a=1
\]
\[
b=2\cdot1+2=4
\]
因此 \([F]=1,\ [G]=4\)。