# H30-2-II-1 解答

## (1)
\[
b_n=\frac{n+1}{3^n a_n}
\Rightarrow
\frac{b_n}{b_{n-1}}
=\frac{n+1}{n}\cdot\frac{1}{3}\cdot\frac{a_{n-1}}{a_n}
=\frac{n+1}{3n}\cdot\frac{a_{n-1}}{a_n}
\]
よって **A=2（n+1）, B=8（3n）**。

与式より
\[
\frac{a_{n-1}}{a_n}=\frac{3n(2n+1)}{(n+1)(2n-3)}
\]
したがって
\[
\frac{b_n}{b_{n-1}}=\frac{2n+1}{2n-3}
\]
より **C=4（2n+1）, D=5（2n-3）**。

これを用いると
\[
a_n=\frac{n+1}{3^n(2n-1)(2n+1)}
\]
なので **E=3（2n-1）**。

## (2)
\[
c_{n-1}=\frac{1}{3^{n-1}(2n-1)}=\frac{3}{3^n(2n-1)},\quad
c_n=\frac{1}{3^n(2n+1)}
\]
\[
a_n=\frac{n+1}{3^n(2n-1)(2n+1)}
=\frac14c_{n-1}-\frac14c_n
\]
よって **F=1, G=4, HI=-1, J=4**。

\[
S_n=\sum_{k=1}^n a_k=\frac14(c_0-c_n)=\frac14(1-c_n)
\]
より **K=1, L=4, M=1**。

\[
\sum_{n=1}^\infty a_n=\lim_{n\to\infty}S_n=\frac14
\]
よって **N=4, O=1**。

## AI解答
A=2,B=8,C=4,D=5,E=3,F=1,G=4,HI=-1,J=4,K=1,L=4,M=1,N=4,O=1
