### I-1（2つの2次関数）

与えられた
\[
f(x)=-2x^2,\qquad g(x)=x^2+ax+b
\]
について条件を用いる。

#### (1)
(i) \(g(x)\) は \(x=3\) で最小  
2次関数 \(x^2+ax+b\) の頂点は \(x=-\frac a2\) なので
\[
-\frac a2=3 \Rightarrow a=-6
\]
よって \([A]=6\)。

(ii) \(g(4)=f(4)\)  
\[
f(4)=-2\cdot 16=-32
\]
\[
g(4)=16+4a+b=16+4(-6)+b=-8+b
\]
\[
-8+b=-32 \Rightarrow b=-24
\]
よって \([BC]=24\)。

最小値は頂点で
\[
g(3)=9+3a+b=9+3(-6)-24=9-18-24=-33
\]
よって最小値 \(-[DE]\) から \([DE]=33\)。

#### (2)
\[
f(x)=g(x)\Rightarrow -2x^2=x^2-6x-24
\]
\[
3x^2-6x-24=0\Rightarrow x^2-2x-8=0
\]
より \([F]=2,[G]=8\)。解は \(x=4,-2\) なので、4と異なる解は \(x=-2\)。  
従って \([H]=2\)。

#### (3)
\[
f(x)-g(x)=-2x^2-(x^2-6x-24)=-3x^2+6x+24
\]
下に凸なので最大は頂点
\[
x=-\frac{6}{2(-3)}=1
\]
よって \([I]=1\)。

最大値は
\[
-3(1)^2+6(1)+24=27
\]
従って \([JK]=27\)。
