Ⅱ

问1　数列 \(\{a_n\}\) 是

\[
a_1=\frac{2}{9},\quad a_n=\frac{(n+1)(2n-3)}{3n(2n+1)}a_{n-1}\quad (n=2,3,4,\cdots)
\]

已知······。此时，求一般项 \(a_n\) 与无限级数 \(\displaystyle \sum_{n=1}^{\infty}a_n\) 的和。

（1）在下文的 \(\boxed{A}\) ～ \(\boxed{E}\) 中，请从下面的选项0～9中选择合适的答案。

首先，设定\(
b_n=\frac{n+1}{3^n a_n}
\)，将\(
\frac{b_n}{b_{n-1}}
\)用\(n\)的式子表示

\[
\frac{b_n}{b_{n-1}}
=\frac{\boxed{A}}{\boxed{B}}\cdot\frac{a_{n-1}}{a_n}
=\frac{\boxed{C}}{\boxed{D}}
\]

成为。由此式

\[
a_n=\frac{n+1}{3^n\boxed{E}(2n+1)}
\]

是。

　　　　　　　　　　　
　　　　　　　　
⓪ \(n-1\)　　① \(n\)　　　② \(n+1\)　　　③ \(2n-1\)　　　④ \(2n+1\)  
⑤ \(2n-3\)　　　⑥ \(2n+3\)　　　⑦ \(3n-1\)　　　⑧ \(3n\)　　　⑨ \(3n+1\)

（2）接下来，设\(
c_n=\frac{1}{3^n(2n+1)}\quad (n=0,1,2,\cdots)
\)。此时，设\(a_n=Ac_{n-1}+Bc_n\)，则有\(
A=\frac{\boxed{F}}{\boxed{G}},\quad B=\frac{\boxed{HI}}{\boxed{J}}
\)。利用此式，可求得\(
S_n=\sum_{k=1}^{n}a_k
\)。

\[
S_n=\frac{\boxed{K}}{\boxed{L}}\left(\boxed{M}-c_n\right)
\]

成为。因此。

\[
\sum_{n=1}^{\infty}a_n=\lim_{n\to\infty}S_n=\frac{\boxed{N}}{\boxed{O}}
\]

获得。