令
\[
t=\log_3 x.
\]
则
\[
\log_3(3x)=t+1,\quad \log_3(9x)=t+2,\quad \log_{1/3}x=-t,\quad \log_{1/3}27=-3.
\]
所以
\[
f(x)=2(t+1)^3+a(t+2)^2-bt-3.
\]
展开：
\[
2(t+1)^3=2t^3+6t^2+6t+2,\quad a(t+2)^2=at^2+4at+4a.
\]
故
\[
f(x)=2t^3+(a+6)t^2+(4a-b+6)t+(4a-1).
\]
因此
\[
A=2,\ B=6,\ C=4,\ D=6,\ E=4,\ F=1.
\]
记
\[
g(t)=2t^3+(a+6)t^2+(4a-b+6)t+(4a-1),
\]
则
\[
g'(t)=6t^2+2(a+6)t+(4a-b+6).
\]
因此
\[
G=6,\ H=2.
\]

---

## 利用极大值点求 \(b\)

题设：\(x=\frac19\) 处极大。此时
\[
t=\log_3\left(3^{-2}\right)=-2.
\]
故
\[
IJ=-2,\quad g'(-2)=0.
\]
代入：
\[
g'(-2)=6\cdot4+2(a+6)(-2)+(4a-b+6)
=24-4(a+6)+4a-b+6
=6-b.
\]
令其为 0，得
\[
b=6,
\]
即
\[
K=6.
\]

---

## 因数分解与极小值点

将 \(b=6\) 代回：
\[
g'(t)=6t^2+2(a+6)t+4a=2(3t+a)(t+2).
\]
因此
\[
L=2,\ M=3,\ N=2.
\]

题设：在 \(x=k\)（即 \(t=p=\log_3 k\)）处取极小值，且 \(p> -2\)。  
由于极大点已在 \(t=-2\)，另一个驻点 \(t=-a/3\) 必为极小点：
\[
p=-\frac{a}{3}\quad\Rightarrow\quad a=-3p.
\]

---

## 代入极小值为 -20 求 \(p\)

当 \(b=6\) 时，
\[
g(t)=2t^3+(a+6)t^2+4at+(4a-1).
\]
代入 \(t=p,\ a=-3p\)：
\[
g(p)=2p^3+(-3p+6)p^2+4(-3p)p+4(-3p)-1
=-(p^3+6p^2+12p+1).
\]
令 \(g(p)=-20\) 得
\[
p^3+6p^2+12p+1=20
\Rightarrow p^3+6p^2+12p-19=0.
\]
注意
\[
(p+2)^3=p^3+6p^2+12p+8,
\]
故上式等价于
\[
(p+2)^3=27 \Rightarrow p+2=3 \Rightarrow p=1.
\]
因此
\[
T=1.
\]

于是
\[
a=-3p=-3 \Rightarrow X=3.
\]
且
\[
k=3^p=3 \Rightarrow Y=3.
\]
