# H18-1 IV 問1

## 题意
\[
f(x)=x(x-1)^{3/2},\quad g(x)=\frac{5+\log x}{1+\log x},\quad h(x)=f(g(x))
\]
求 \(f'(x),g'(x),h'(x)\) 的指定形式填空。（\(\log\) 为自然对数）

---

## 解法

### 1) 计算 \(f'(x)\)
\[
f(x)=x(x-1)^{3/2}
\]
乘积求导：
\[
f'(x)=(x-1)^{3/2}+x\cdot \frac{3}{2}(x-1)^{1/2}
\]
提取 \((x-1)^{1/2}\)：
\[
f'(x)=(x-1)^{1/2}\left((x-1)+\frac{3}{2}x\right)
=(x-1)^{1/2}\left(\frac{5}{2}x-1\right)
=\frac12 (x-1)^{1/2}(5x-2)
\]
因此
\[
A=1,\ B=2,\ C=5,\ D=2.
\]

### 2) 计算 \(g'(x)\)
\[
g(x)=\frac{5+\log x}{1+\log x}
\]
设 \(u=5+\log x,\ v=1+\log x\)，则 \(u'=v'=\frac1x\)。
\[
g'(x)=\frac{u'v-uv'}{v^2}=\frac{1}{x}\cdot\frac{v-u}{v^2}
=\frac{1}{x}\cdot\frac{(1+\log x)-(5+\log x)}{(1+\log x)^2}
=-\frac{4}{x(1+\log x)^2}
\]
因此 \(E=4,\ F=2\)。

### 3) 计算 \(h'(x)\)
\[
h'(x)=f'(g(x))\cdot g'(x)
\]
先算：
\[
g(x)-1=\frac{5+\log x}{1+\log x}-1=\frac{4}{1+\log x}
\Rightarrow \sqrt{g(x)-1}=\frac{2}{(1+\log x)^{1/2}}
\]
以及：
\[
5g(x)-2=\frac{5(5+\log x)-2(1+\log x)}{1+\log x}
=\frac{23+3\log x}{1+\log x}
\]
所以
\[
f'(g(x))=\frac12\sqrt{g(x)-1}\,(5g(x)-2)
=\frac12\cdot \frac{2}{(1+\log x)^{1/2}}\cdot\frac{23+3\log x}{1+\log x}
=\frac{23+3\log x}{(1+\log x)^{3/2}}
\]
再乘上
\[
g'(x)=-\frac{4}{x(1+\log x)^2}
\]
得到
\[
h'(x)=-\frac{4(23+3\log x)}{x(1+\log x)^{7/2}}
\]
因此
\[
GH=23,\ I=3,\ \frac{J}{K}=\frac{7}{2}.
\]

---

## 答案
\[
A=1,\ B=2,\ C=5,\ D=2,\ E=4,\ F=2,\ GH=23,\ I=3,\ \frac{J}{K}=\frac{7}{2}
\]