# H23-2-IV-1

## (1)
\[
f(x)=4\sqrt3 e^{-x}\cos x+6e^{-x}=2e^{-x}(2\sqrt3\cos x+3)
\]
\(e^{-x}>0\) なので
\[
2\sqrt3\cos x+3=0\Rightarrow \cos x=-\frac{\sqrt3}{2}
\]
\[
0\le x<2\pi \Rightarrow a=\frac{5\pi}{6},\ b=\frac{7\pi}{6}
\]
よって \(A/B=5/6,\ C/D=7/6\)。

## (2)
\[
\frac{d}{dx}\bigl(pe^{-x}\cos x+qe^{-x}\sin x\bigr)
=e^{-x}\{(-p+q)\cos x-(p+q)\sin x\}
\]
これが \(e^{-x}\cos x\) に等しいので
\[
-p+q=1,\quad p+q=0 \Rightarrow p=-\frac12,\ q=\frac12
\]
よって \(EF/G=-1/2,\ H/I=1/2\)。

## (3)
\[
\int e^{-x}\cos x\,dx=-\frac12 e^{-x}(\cos x+\sin x)
\]
\[
\int f(x)\,dx=-2\sqrt3 e^{-x}(\cos x+\sin x)-6e^{-x}
\]
\(A=e^{-a},B=e^{-b}\) とおくと計算より
\[
\int_a^b f(x)\,dx=(3+\sqrt3)A-(3-\sqrt3)B
\]

