## III

\(a,\ b,\ k\) 为常数。函数

\[
f(x)=2(\log_3 3x)^3+a(\log_3 9x)^2+b\log_{\frac{1}{3}}x+\log_{\frac{1}{3}}27
\]

在 \(x=\dfrac{1}{9}\) 取得极大值，在 \(x=k\) 取得极小值 \(-20\)。  
此时，求 \(a,\ b,\ k\) 的值。

假设 \(t=\log_3 x\)，\(f(x)\) 使用 \(t\)

\[
f(x)=\boxed{A}t^3+(a+\boxed{B})t^2+(\boxed{C}a-b+\boxed{D})t+\boxed{E}a-\boxed{F}
\]

如上所示。若将此式记作 \(g(t)\)，则 \(g(t)\) 的导函数 \(g'(t)\) 为

\[
g'(t)=\boxed{G}t^2+\boxed{H}(a+\boxed{B})t+\boxed{C}a-b+\boxed{D}
\]

是。根据假设，\(g(t)\) 在 \(t=\boxed{IJ}\) 取得极大值，所以 \(g'(\boxed{IJ})=0\)。由此可得，\(b=\boxed{K}\)。因此

\[
g'(t)=\boxed{L}\,(\boxed{M}t+a)(t+\boxed{N})
\]

并被因式分解。

设 \(\log_3 k=p\)，\(g(t)\) 在 \(t=p\) 处取得极小值 \(-20\)，所以，由 \(g'(p)=0\) 且 \(p>\boxed{IJ}\)，可得 \(a=-\boxed{M}p\)。将其代入 \(g(p)=-20\) 并整理后，

\[
p^3+\boxed{O}p^2+\boxed{PQ}p-\boxed{RS}=(p-\boxed{T})(p^2+\boxed{U}p+\boxed{VW})=0
\]

表示为。\(p^2+\boxed{U}p+\boxed{VW}\) 因为始终为正，所以得到 \(p=\boxed{T}\)。因此

\[
a=-\boxed{X},\qquad k=\boxed{Y}
\]

是。