### II-1 解析

等差：\(a_n=c+(n-1)d\)，等比：\(b_n=cd^{n-1}\)，且 \(d>0\)。

#### (1)
由 \(a_5=b_3,\ a_7=b_5\)：
\[
c+4d=cd^2,\qquad c+6d=cd^4.
\]
因此 \(A=4,\ B=2,\ C=6,\ D=4\)。

消去 \(c\)：
\[
c=\frac{4d}{d^2-1}=\frac{6d}{d^4-1}.
\]
约去 \(d\neq0\)，得
\[
4(d^4-1)=6(d^2-1)\Rightarrow 2d^4-3d^2+1=0.
\]
令 \(t=d^2\)：
\[
2t^2-3t+1=(2t-1)(t-1)=0.
\]
\(t=1\) 会导致原式矛盾（分母为0），舍去；故 \(t=\frac12\)，
\[
d=\sqrt{\frac12}=\frac{\sqrt2}{2}.
\]
所以 \(E=2,\ F=2\)。

代回 \(c+4d=cd^2\Rightarrow c(1-d^2)=-4d\)：
\[
c=\frac{-4d}{1-d^2}=\frac{-4(\sqrt2/2)}{1-1/2}=-4\sqrt2.
\]
故 \(c= GH \sqrt{I} \) 中 \(GH=-4,\ I=2\)。

#### (2)
\(d=2^{-1/2}\)，\(c=-4\sqrt2\)：
\[
b_n=cd^{n-1}=-4\sqrt2\cdot 2^{-(n-1)/2}.
\]
当 \(n\) 为偶数 \(n=2k\) 时，上式为 \(-8\cdot 2^{-k}\)，为有理数；奇数项为无理数。

因此有理项为 \(b_2,b_4,\dots,b_{2m}\)：
\[
\sum_{k=1}^m b_{2k}=\sum_{k=1}^m\left(-8\cdot 2^{-k}\right)
=-8\sum_{k=1}^m\left(\frac12\right)^k
=-8\left(1-\left(\frac12\right)^m\right)
=8\left(\left(\frac12\right)^m-1\right).
\]
故 \(J=8,\ K=1,\ L=2,\ M=1\)。

**填空：**  
\(A=4,\ B=2,\ C=6,\ D=4,\ E=2,\ F=2,\ GH=-4,\ I=2,\ J=8,\ K=1,\ L=2,\ M=1\)。
