### I-1 解析

设 \(6-\sqrt5\) 的整数部分为 \(a\)，小数部分为 \(b\)，则 \(6-\sqrt5=a+b,\ 0\le b<1\)。

1. \(\sqrt5\approx2.236\)，所以 \(6-\sqrt5\approx3.763\)，因此
\[
a=3,\qquad b=(6-\sqrt5)-3=3-\sqrt5.
\]

2. 计算
\[
\frac{4}{b}=\frac{4}{3-\sqrt5}=\frac{4(3+\sqrt5)}{(3-\sqrt5)(3+\sqrt5)}
=\frac{4(3+\sqrt5)}{9-5}=3+\sqrt5,
\]
故
\[
b+\frac4b=(3-\sqrt5)+(3+\sqrt5)=6.
\]

3. 用恒等式 \(x^3+y^3=(x+y)^3-3xy(x+y)\)，令 \(x=b,\ y=4/b\)，则 \(xy=4\)，
\[
b^3+\left(\frac4b\right)^3=\left(b+\frac4b\right)^3-12\left(b+\frac4b\right).
\]

4. 代入 \(b+4/b=6\)：
\[
b^3+\left(\frac4b\right)^3=6^3-12\cdot6=216-72=144.
\]
又 \(4a^3=4\cdot 3^3=108\)，所以
\[
4a^3-\left\{b^3+\left(\frac4b\right)^3\right\}=108-144=-36.
\]

**填空：**  
\(A=3,\ B=6,\ C=3,\ DE=12,\ FGH=-36\)。
