## IV　问题2

数列 \(\{a_n\}\)

\[
a_n = \int_{0}^{\frac{1}{4}} x^n e^{-x}\,dx \qquad (n = 1,2,3,\ldots)
\]

规定。

此时

\[
a_1 = -\frac{\boxed{H}}{\boxed{I}}\,e^{\frac{\boxed{JK}}{\boxed{L}}} + 1
\]

是。

另外，\(a_{n+1}\) 使用 \(a_n\)

\[
a_{n+1} = -\left(\frac{\boxed{M}}{\boxed{N}}\right)^{n+1} e^{\frac{\boxed{JK}}{\boxed{L}}}+ (n + \boxed{O})a_n
\qquad (n = 1,2,3,\ldots)
\]

被表示为。若对其进行变形，

\[
na_n = a_{n+1} - a_n + \left(\frac{\boxed{M}}{\boxed{N}}\right)^{n+1} e^{\frac{\boxed{JK}}{\boxed{L}}}
\]

旁边

\[
\sum_{k=1}^{n} ka_k = a_{n+1} - a_1 + \frac{\boxed{P}}{\boxed{QR}}\,e^{\frac{\boxed{JK}}{\boxed{L}}}
\left\{1 - \left(\frac{\boxed{S}}{\boxed{T}}\right)^{n}\right\}
\]

得到。

这里，\(0 \le x\) 时，\(e^{-x}\) 的取值范围是   \(0 < e^{-x} \le \boxed{U}\)，因为

\[
0 < a_n
< \int_{0}^{\frac{1}{4}} \boxed{U}\,x^n\,dx
= \frac{1}{\boxed{V}^{\,n+1}(n+1)}
\]

成立。 因此

\[
\lim_{n\to\infty} a_n = \boxed{W}
\]

因为

\[
\lim_{n\to\infty} \sum_{k=1}^{n} ka_k
= \frac{\boxed{X}}{\boxed{Y}}\,e^{\frac{\boxed{JK}}{\boxed{L}}} - 1
\]

获得。