# H20-2-I-2 解答

## (1) 因数分解
\[
P=6ab+9a-4b-6=3a(2b+3)-2(2b+3)=(3a-2)(2b+3)
\]
故
\[
[N]=3,\ [O]=2,\ [P]=2,\ [Q]=3
\]

## (2) 代入求 b
给定 \(a=\frac{\sqrt6}{3}\)，则 \(3a=\sqrt6\)，所以
\[
P=(3a-2)(2b+3)=(\sqrt6-2)(2b+3)=\sqrt3-\sqrt2
\]
\[
2b+3=\frac{\sqrt3-\sqrt2}{\sqrt6-2}
\]
有理化（或直接化简）得
\[
\frac{\sqrt3-\sqrt2}{\sqrt6-2}=\frac{\sqrt2}{2}
\]
因此
\[
2b=\frac{\sqrt2}{2}-3=\frac{\sqrt2-6}{2}\Rightarrow b=\frac{\sqrt2-6}{4}
\]
故
\[
[R]=2,\ [S]=6,\ [T]=4
\]

## (3) 整数解
\[
(3a-2)(2b+3)=17
\]
17 为素数，考虑因子分解：

- \(3a-2=1,\ 2b+3=17 \Rightarrow a=1,\ b=7\)
- \(3a-2=-17,\ 2b+3=-1 \Rightarrow a=-5,\ b=-2\)

所以两组为
\[
(a,b)=(1,7),\quad (a,b)=(-5,-2)
\]
对应 \([U]=1,[V]=7,[WX]=-5,[YZ]=-2\)。
