### III-2（对数不等式 → 代数不等式）

给定
\[
2\log_3(x-y)\le \log_3 x+\log_3 y.
\]

**真数条件：**
\[
x>0,\ y>0,\ x-y>0 \Rightarrow 0<\frac{y}{x}<1.
\]
故 \([N]=0,\ [O]=1\)。

**变形①：** 因 \(\log_3\) 单调递增，
\[
2\log_3(x-y)\le \log_3 x+\log_3 y
\iff \log_3 (x-y)^2\le \log_3(xy)
\iff (x-y)^2\le xy.
\]
展开：
\[
x^2-2xy+y^2\le xy \Rightarrow x^2-3xy+y^2\le 0.
\]
故 \([P]=3,\ [Q]=0\)。

令 \(t=\dfrac{y}{x}\)（因 \(x>0\) 可除），得
\[
1-3t+t^2\le 0 \iff t^2-3t+1\le 0.
\]
解方程 \(t^2-3t+1=0\)：
\[
t=\frac{3\pm\sqrt5}{2}.
\]
故
\[
\frac{3-\sqrt5}{2}\le t\le \frac{3+\sqrt5}{2}.
\]
再与 \(0<t<1\) 取交集，得到
\[
\frac{3-\sqrt5}{2}\le \frac{y}{x}<1.
\]
对应填空：
\[
[R]=3,\ [S]=5,\ [T]=2,\ [U]=1.
\]
