### II-2（等差数列求和与不等式）

等差数列 \(a_1=x\)，公差 \(-1\)，故
\[
a_n=x-(n-1).
\]

**基础式**
\[
a_{2k-1}=x-(2k-2),\quad a_{2k+1}=x-2k
\]
\[
a_{2k-1}-a_{2k+1}=2\Rightarrow [J]=2.
\]
又
\[
a_{2k}=x-(2k-1)=x+1-2k
\]
\[
a_{2k}^2=(x+1-2k)^2=(x+1)^2-4k(x+1)+4k^2
\Rightarrow [K]=4,\ [L]=4.
\]

---

#### (1) 计算 \(\dfrac{T_n}{2n}\)

\[
T_n=\sum_{k=1}^n (a_{2k-1}-a_{2k+1})a_{2k}^2
=\sum_{k=1}^n 2a_{2k}^2.
\]
令 \(y=x+1\)，则
\[
\frac{T_n}{2n}=\frac1n\sum_{k=1}^n (y-2k)^2
=\frac1n\sum (y^2-4ky+4k^2).
\]
用
\[
\sum_{k=1}^n k=\frac{n(n+1)}2,\quad
\sum_{k=1}^n k^2=\frac{n(n+1)(2n+1)}6
\]
得
\[
\frac{T_n}{2n}=y^2-2(n+1)y+\frac23(n+1)(2n+1).
\]
与题目形式对应：
\[
[M]=2,\ [N]=1,\ \frac{[O]}{[P]}=\frac23\Rightarrow [O]=2,[P]=3,
\]
\[
(n+[Q])=(n+1)\Rightarrow [Q]=1,\quad ([R]n+1)=(2n+1)\Rightarrow [R]=2.
\]

---

#### (2) 由 \(T_8<352\) 求 \(x\) 及 \(a_8\)

取 \(n=8\)：
\[
\frac{T_8}{16}=(x+1)^2-18(x+1)+80.
\]
\(T_8<352\iff \frac{T_8}{16}<22\)：
\[
(x+1)^2-18(x+1)+58<0.
\]
等价于
\[
y^2-18y+80<0\quad (y=x+1),
\]
根为 \(y=8,10\)，故
\[
8<y<10\Rightarrow 7<x<9.
\]
所以 \([S]=7,\ [T]=9\)。

若 \(x\) 为整数，则 \(x=8\)，于是
\[
a_8=x-7=1,
\]
故 \([U]=1\)。
