### (1)
令 \(y=\dfrac{x}{2}\)，则
\[
\left(\frac{x}{2}+1\right)\left(\frac{x}{2}+2\right)\left(\frac{x}{2}+3\right)\left(\frac{x}{2}+4\right)
=(y+1)(y+2)(y+3)(y+4).
\]
配对：
\[
(y+1)(y+4)=y^2+5y+4,\quad (y+2)(y+3)=y^2+5y+6.
\]
相乘得
\[
(y^2+5y+4)(y^2+5y+6)=y^4+10y^3+35y^2+50y+24.
\]
代回 \(y=x/2\)：
\[
\frac{1}{16}x^4+\frac{5}{4}x^3+\frac{35}{4}x^2+25x+24.
\]
故
\[
A=5,\ B=4,\ CD=35,\ E=4.
\]

### (2)
设 \(a=\sqrt2+\sqrt3\)，则
\[
x=a+\sqrt5,\quad y=a-\sqrt5.
\]
因此
\[
xy=(a+\sqrt5)(a-\sqrt5)=a^2-5.
\]
而
\[
a^2=(\sqrt2+\sqrt3)^2=2+3+2\sqrt6=5+2\sqrt6,
\]
所以
\[
xy=2\sqrt6 \Rightarrow F=2,\ G=6.
\]

再算
\[
\frac{x}{y}=\frac{a+\sqrt5}{a-\sqrt5}
=\frac{(a+\sqrt5)^2}{a^2-5}.
\]
分母 \(a^2-5=2\sqrt6\)。分子
\[
(a+\sqrt5)^2=a^2+5+2a\sqrt5=(5+2\sqrt6)+5+2(\sqrt2+\sqrt3)\sqrt5
=10+2\sqrt6+2\sqrt{10}+2\sqrt{15}.
\]
故
\[
\frac{x}{y}=\frac{10+2\sqrt6+2\sqrt{10}+2\sqrt{15}}{2\sqrt6}
=\frac{5+\sqrt6+\sqrt{10}+\sqrt{15}}{\sqrt6}
=1+\frac{5}{6}\sqrt6+\frac{\sqrt{10}}{2}+\frac{\sqrt{15}}{3}.
\]
因此
\[
H=5,\ I=6,\ J=2,\ K=3.
\]
