\[
f(x)=a(2e^{3x}+3e^{-2x})+a^2,\quad a\ne0.
\]

## (1)
\[
f'(x)=a(6e^{3x}-6e^{-2x})\Rightarrow \frac{f'(0)}a=6-6=0.
\]
\[
f''(x)=a(18e^{3x}+12e^{-2x})\Rightarrow \frac{f''(0)}a=18+12=30.
\]
故 \(A=0,\ BC=30\)。

## (2)
设 \(g(x)=2e^{3x}+3e^{-2x}\)，则
\[
g'(x)=6e^{3x}-6e^{-2x}=0\Rightarrow e^{5x}=1\Rightarrow x=0,
\]
且 \(g''(x)>0\)，所以 \(g\) 在 \(x=0\) 取最小值 \(g_{\min}=g(0)=5\)。

若 \(a<0\)，则 \(f(x)=ag(x)+a^2\) 随 \(g(x)\to\infty\) 会趋于 \(-\infty\)，无最小值；  
因此要“有最小值”，必须 \(a>0\)。

于是
\[
f_{\min}=a\cdot 5+a^2=a^2+5a=36
\Rightarrow (a+9)(a-4)=0.
\]
结合 \(a>0\)，得 \(a=4\)，故 \(D=4\)。

此时
\[
f(x)=4(2e^{3x}+3e^{-2x})+16=8e^{3x}+12e^{-2x}+16.
\]
积分：
\[
\int_0^1 8e^{3x}dx=\frac{8}{3}(e^3-1)=\frac{8}{3}e^3-\frac{8}{3},
\]
\[
\int_0^1 12e^{-2x}dx=-6(e^{-2}-1)=6-6e^{-2},
\]
\[
\int_0^1 16dx=16.
\]
合并：
\[
\int_0^1 f(x)dx=\frac{8}{3}e^3-6e^{-2}+\frac{58}{3}.
\]
故
\[
E=8,\ F=3,\ G=6,\ HI=58,\ J=3.
\]
