## I-2  因数分解 → 代入计算

已知  
\(P=2x^2-x+2,\quad Q=x^2-2x+1\)  
\[
E=P^2-4Q^2-3P+6Q
\]

### (1) 用 P,Q 因数分解
\[
E=(P^2-4Q^2)-3(P-2Q)
\]
\[
P^2-4Q^2=(P-2Q)(P+2Q)
\]
所以
\[
E=(P-2Q)\{(P+2Q)-3\}=(P-2Q)(P+2Q-3)
\]

因此  
\[
E=(P-2Q)(P+2Q-3)
\]
对应：\(L=2,\ M=2,\ N=3\)。

### (2) 化为 x 的式子
先算
\[
P-2Q=(2x^2-x+2)-2(x^2-2x+1)=2x
\]
再算
\[
P+2Q-3=(2x^2-x+2)+2(x^2-2x+1)-3=4x^2-5x+1
\]
\[
4x^2-5x+1=(x-1)(4x-1)
\]
故
\[
E=2x(x-1)(4x-1)
\]
对应：\(O=2,\ P=1,\ Q=4,\ R=1\)。

### (3) 代入给定 x
\[
x=-\frac{1-\sqrt5}{3-\sqrt5}
=-\frac{(1-\sqrt5)(3+\sqrt5)}{(3-\sqrt5)(3+\sqrt5)}
=-\frac{(1-\sqrt5)(3+\sqrt5)}{4}
\]
\[
(1-\sqrt5)(3+\sqrt5)=3+\sqrt5-3\sqrt5-5=-2-2\sqrt5
\]
\[
x=\frac{2+2\sqrt5}{4}=\frac12+\frac{\sqrt5}{4}
\]
于是
\[
2x=1+\frac{\sqrt5}{2},\quad x-1=-\frac12+\frac{\sqrt5}{4},\quad 4x-1=1+\sqrt5
\]
计算得
\[
E=2x(x-1)(4x-1)=\frac{15}{4}+\frac{5}{2}\sqrt5
\]
对应：\(S=\dfrac{15}{4},\ T=\dfrac{5}{2},\ U=5\)。
