# H24-1-II 解答

已知
\[
\sum_{k=1}^n a_k = n^2+3n.
\]

## (1)
\[
a_n=\left(\sum_{k=1}^n a_k\right)-\left(\sum_{k=1}^{n-1} a_k\right)
=(n^2+3n)-\{(n-1)^2+3(n-1)\}.
\]
计算：
\[
(n-1)^2+3(n-1)=n^2-2n+1+3n-3=n^2+n-2.
\]
故
\[
a_n=(n^2+3n)-(n^2+n-2)=2n+2.
\]
因此 \([A]=2,\ [B]=2\)。

## (2)
\[
b_n=n^2-5n-6=(n-6)(n+1).
\]
因 \(n+1>0\)，所以 \(b_n<0 \iff n-6<0 \iff n=1,2,3,4,5\)。  
项数为 5，所以 \([C]=5\)。

求和：
\[
b_1=-10,\ b_2=-12,\ b_3=-12,\ b_4=-10,\ b_5=-6,
\]
总和
\[
-10-12-12-10-6=-50.
\]
题面写成 \(-[DE]\)，故 \([DE]=50\)。

## (3)
由(1)得 \(a_k=2(k+1)\)，且
\[
b_k=(k-6)(k+1).
\]
于是
\[
\frac{k^2 b_k}{a_k}=\frac{k^2(k-6)(k+1)}{2(k+1)}=\frac12 k^2(k-6)=\frac12(k^3-6k^2).
\]
所以
\[
\sum_{k=1}^n\frac{k^2 b_k}{a_k}
=\frac12\left(\sum_{k=1}^n k^3-6\sum_{k=1}^n k^2\right).
\]
使用公式
\[
\sum_{k=1}^n k^3=\left(\frac{n(n+1)}2\right)^2,\quad
\sum_{k=1}^n k^2=\frac{n(n+1)(2n+1)}6.
\]
代入并化简得
\[
\sum_{k=1}^n\frac{k^2 b_k}{a_k}
=\frac18\,n(n+1)(n^2-7n-4).
\]
与题给形式比较：
\[
\frac{1}{[F]}n(n+[G])(n^2-[H]n-[I])
\]
可知
\[
[F]=8,\ [G]=1,\ [H]=7,\ [I]=4.
\]
