# H24-2-IV-2 解答

\[
a_n=\int_0^{1/4} x^n e^{-x}\,dx.
\]

(1) \(a_1\)：
\[
\int x e^{-x}dx=-(x+1)e^{-x}+C
\Rightarrow a_1=\Bigl[-(x+1)e^{-x}\Bigr]_0^{1/4}
=-\frac54 e^{-1/4}+1.
\]
故 \([H]=5,[I]=4,[JK]=-1,[L]=4\)。

(2) 递推（分部积分）：
\[
a_{n+1}=\int_0^{1/4} x^{n+1}e^{-x}dx
=\Bigl[-x^{n+1}e^{-x}\Bigr]_0^{1/4}+(n+1)\int_0^{1/4}x^n e^{-x}dx
=-(1/4)^{n+1}e^{-1/4}+(n+1)a_n.
\]
故 \([M]=1,[N]=4,[O]=1\)。

变形得
\[
na_n=a_{n+1}-a_n+(1/4)^{n+1}e^{-1/4}.
\]
求和：
\[
\sum_{k=1}^n k a_k=a_{n+1}-a_1+e^{-1/4}\sum_{k=1}^n (1/4)^{k+1}.
\]
几何级数
\[
\sum_{k=1}^n (1/4)^{k+1}=\frac{1}{16}\cdot\frac{1-(1/4)^n}{1-1/4}
=\frac{1}{12}\left(1-(1/4)^n\right).
\]
故 \([P]=1,[QR]=12,[S]=1,[T]=4\)。

(3) 因 \(x\ge0\Rightarrow 0<e^{-x}\le1\)，故 \([U]=1\)。
于是
\[
0<a_n<\int_0^{1/4} x^n dx=\frac{(1/4)^{n+1}}{n+1}=\frac{1}{4^{n+1}(n+1)},
\]
故 \([V]=4\)，从而 \(\lim_{n\to\infty}a_n=0\Rightarrow [W]=0\)。

(4) 取极限：
\[
\lim_{n\to\infty}\sum_{k=1}^n k a_k=0-a_1+\frac{1}{12}e^{-1/4}
=-1+\left(\frac54+\frac{1}{12}\right)e^{-1/4}
=-1+\frac43 e^{-1/4}.
\]
故 \([X]=4,[Y]=3\)。
