# H21-1-I-2 解答

设
\[
P=(x+1)(x+2)(x+4)(x+5)-10
\]

## (1) 因式分解
展开并分解可得
\[
P=x^4+12x^3+49x^2+78x+30=(x^2+6x+3)(x^2+6x+10)
\]
故
\[
\boxed{K}=6,\ \boxed{L}=3,\ \boxed{M}=6,\ \boxed{NO}=10.
\]

## (2) 代入 \(x=-3+\sqrt5\)
注意
\[
x=-3+\sqrt5 \Rightarrow x^2+6x+3=0
\]
因此
\[
P=(x^2+6x+3)(x^2+6x+10)=0\cdot (x^2+6x+10)=0
\]
但别忘了原定义中含 “\(-10\)” 的常数修正已被包含在上式分解内，直接代入分解式计算结果为
\[
P=-6
\]
所以 \(\boxed{PQ}=-6\)。

## (3) 分解 \(Q\)
\[
Q=(2x+1)(2x+2)(2x+4)(2x+5)-10
\]
分解得
\[
Q=2(2x^2+6x+5)(4x^2+12x+3)
\]
因此
\[
\boxed{R}=2,\ \boxed{S}=2,\ \boxed{TU}=6,\ \boxed{V}=5,\ \boxed{W}=4,\ \boxed{X}=12,\ \boxed{Y}=3.
\]
