## II-2 数列 {a_n}

已知 \(a_n>0\)，且
\[
4\sqrt{S_n}=a_n+4,\quad S_n=\sum_{k=1}^n a_k
\]

### (1) 求 \(a_1\)
\(S_1=a_1\)，故
\[
4\sqrt{a_1}=a_1+4
\]
令 \(\sqrt{a_1}=t>0\)，则 \(4t=t^2+4\Rightarrow (t-2)^2=0\Rightarrow t=2\)。  
\[
a_1=4
\]
故 **K=4**。

---

### (2) 求 \(a_{n+1}-a_n\)
由 \(4\sqrt{S_n}=a_n+4\Rightarrow S_n=\dfrac{(a_n+4)^2}{16}\)。

又
\[
S_{n+1}=S_n+a_{n+1}
\]
所以
\[
\frac{(a_{n+1}+4)^2}{16}=\frac{(a_n+4)^2}{16}+a_{n+1}
\]
\[
(a_{n+1}+4)^2-(a_n+4)^2=16a_{n+1}
\]
故 **LM=16，N=4，O=4**。

设 \(b_n=a_n+4\)，则
\[
b_{n+1}^2=b_n^2+16b_{n+1}-64
\Rightarrow (b_{n+1}-8)^2=b_n^2
\]
且 \(b_1=a_1+4=8>0\)，取正号得
\[
b_{n+1}-8=b_n\Rightarrow b_{n+1}=b_n+8
\]
所以 \(b_n=8n\)，
\[
a_n=b_n-4=8n-4
\]
从而
\[
a_{n+1}-a_n=8
\]
故 **P=8**。

---

### (3)
\[
a_n=68\Rightarrow 8n-4=68\Rightarrow 8n=72\Rightarrow n=9
\]
故 **Q=9**。
